\leveldown{Properties of Wiener Process - pg. 80}

\leveldown{Problem}

From pg 80, prove for the Wiener process that
\begin{equation*}
\avg{Y(t_1) Y(t_2)} = \min(t_1, t_2)
\end{equation*}

\begin{equation*}
\avg{ \big( Y(t_1) - Y(t_2) \big)  \big( Y(t_3) - Y(t_4) \big) } = \big( t_1, t_2 \big) \cap \big( t_3, t_4 \big)
\end{equation*}

These are equations $(2.7a)$ and $(2.7b)$ in the textbook, respectively.

\levelstay{Solution}

Let $t_1 < t_2$. Then the joint density of $Y (t_1)$ and  $Y (t_2)$ is 

\begin{equation*}
f_{Y (t_1)Y(t_2)} = p(t_1, 0, x)p(t_2 - t_1, x, y)dxdy
\end{equation*}
for their respective probability distributions. Then, 

\begin{align*}
\avg{Y(t_1)Y(t_2)} =& \int_{-\infty}^{\infty} \int_{-\infty}^{\infty} x y p(t_1, 0, x)p(t_2 - t_1, x, y)dxdy \\
= & \int_{-\infty}^{\infty} x p(t_1, 0, x) \bigg( \int_{-\infty}^{\infty} y p(t_2 - t_1, x, y)dy \bigg) dx\\
= & \int_{-\infty}^{\infty} x p(t_1, 0, x) \bigg( \int_{-\infty}^{\infty} y p(t_2 - t_1, x, y)dy \bigg) dx .
\end{align*}

where in the last step we have used Fubini's/Tonelli's theorem. 

The integral in brackets is given by: 

\begin{align*}
\int_{-\infty}^{\infty} y p(t_2 - t_1, x, y)dy =& \int_{-\infty}^{\infty} (x + u) p(t_2 - t_1, x, x + u)du \\
= & \int_{-\infty}^{\infty} (x + u) p(t_2 - t_1, 0, u)du \\
= & x \underbrace{ \int_{-\infty}^{\infty} p(t_2 - t_1, 0, u)du }_1 + \int_{-\infty}^{\infty} u p(t_2 - t_1, 0, u)du \\
= & x + 0 .
\end{align*}

where in the first line we have used the substitution $y = x + u$ so that $dy = du$ and in the second line we have used the fact that length of an interval is invariant under shifts, e.g. for some real number $x$, the length of interval, given by $length(\big[a, b \big]) = b - a$, for the interval $ \big[x, x + u  \big] $ is $(x + u) - x = u$ which is the same length as the interval $ \big[0, u  \big] $ (which has length $(u - 0) = u$ ). So in the second-last line, the first integral is $x$ while the second integral is $0$.

Putting this into our new equation gives 

\begin{align*}
\int_{-\infty}^{\infty} x p(t_1, 0, x) \underbrace{ \bigg( \int_{-\infty}^{\infty} y p(t_2 - t_1, x, y)dy \bigg) }_x dx =& \int_{-\infty}^{\infty} x p(t_1, 0, x) \big( x \big) dx \\
= & \int_{-\infty}^{\infty} x^2 p(t_1, 0, x) dx\\
= & t_1 .
\end{align*}

because the integral in the second line is the expectation integral for the Wiener process which just gives $t_1$.

Therefore for arbitrary $t_2$ and $t_1$, 

\begin{equation*}
\avg{Y(t_1)Y(t_2)} = \min(t_1, t_2)
\end{equation*}

Now we have for the second part, 

\begin{align*}
\avg{ \big( Y(t_1) - Y(t_2) \big)  \big( Y(t_3) - Y(t_4) \big) } =& \avg{ Y(t_1)Y(t_3) - Y(t_1)Y(t_4) - Y(t_2)Y(t_3) + Y(t_2)Y(t_4) } \\
= & \avg{Y(t_1)Y(t_3) } - \avg{Y(t_1)Y(t_4)} - \avg{Y(t_2)Y(t_3)} + \avg{ Y(t_2)Y(t_4)}  \\
= & \min{(t_1,t_3)} - \min{(t_1,t_4)} - \min{(t_2,t_3)} + \min{(t_1,t_3)}  \\
= & \big( t_1, t_2 \big) \cap \big( t_3, t_4 \big)
\end{align*}

where in the second line we have used the linearity of the expectation (i.e. $\avg{ X - Y } = \avg{X} - \avg{Y}$ for random variables X and Y (i.i.d))  and in the third line we have applied the first part of this question to each expectation separately. 