\leveldown{Moments of Gaussian distribution - pg. 5}

\leveldown{Problem}

The \emph{Gauss distribution} is defined by
\begin{equation*}
  P(x) = \frac{1}{\sqrt{2\pi \sigma^2}} \exp \left[ - \frac{x^2}{2 \sigma^2} \right]
  \, .
\end{equation*}
Show that $\mu_{2n+1} = 0$ and
\begin{equation*}
  \mu_{2n} = \sigma^{2n} (2n-1)!! = \sigma^{2n} (2n-1)(2n-3)(2n-5)\cdots 1
  \, .
\end{equation*}

\levelstay{Solution}

The odd moments are obviously zero by symmetry.
For the even moments, first note that $\mu_0 = 1$ is just a statement that the distribution is normalized.
Now consider $\mu_2$,
\begin{align*}
  \mu_{2n}
  &= \frac{1}{\sqrt{2\pi \sigma_2}} \int_{-\infty}^\infty x^{2n} \exp \left[ - \frac{x^2}{2 \sigma^2} \right] \, dx \\
  &= \frac{1}{\sqrt{2 \pi \sigma^2}}
  \left(
    \underbrace{
      \left. \frac{x^{2n + 1}}{2n+1} \exp \left[ - \frac{x^2}{2 \sigma^2} \right]
      \right\rvert_{-\infty}^\infty
    }_0
    + \frac{1}{\sigma^2 (2n + 1)}
    \int_{-\infty}^\infty x^{2n+2} \exp \left[ - \frac{x^2}{2 \sigma^2} \right] \, dx
  \right) \\
  &= \frac{1}{\sigma^2 (2n + 1)} \mu_{2n + 2} \\
  \mu_{2n + 2} &= \sigma^2 (2n + 1) \mu_{2n}
  \, . \tag{$\star$}
\end{align*}
Now use induction.
Assuming the target relation is true for $\mu_{2n}$, we can rewrite $(\star)$ as
\begin{align*}
  \mu_{2n + 2} &= \sigma^2 (2n + 1) \sigma^{2n} (2n - 1)(2n - 3)\cdots 1 \\
  \mu_{2n} &= \sigma^{2n} (2n - 1)(2n - 3) \cdots 1
\end{align*}
which is what we wanted to prove.
